venom/props/callLayoutPropsScript.sml
@@ -84,4 +84,72 @@ Proof
   EVAL_TAC
 QED
 
+
+Definition layout_test_fn_with_abi_def:
+  layout_test_fn_with_abi entry_insts other_blocks has_mem_ret user_returns =
+    layout_test_fn entry_insts other_blocks with
+      fn_call_abi := <|
+        ica_has_memory_return_buffer := has_mem_ret;
+        ica_user_return_count := user_returns
+      |>
+End
+
+Theorem raw_return_user_arity_eval:
+  raw_return_user_arity (mk_inst 10 RET [Var "rpc"] []) = SOME 0 /\
+  raw_return_user_arity
+    (mk_inst 11 RET [Var "u0"; Var "u1"; Var "rpc"] []) = SOME 2 /\
+  raw_return_user_arity
+    (mk_inst 12 RETFMP [Var "u0"; Var "rpc"] []) = SOME 1 /\
+  raw_return_user_arity
+    (mk_inst 13 DRET
+      [Lit 1w; Var "ordinary"; Var "src"; Lit 32w; Var "rpc"] []) =
+      SOME 2 /\
+  raw_return_user_arity (mk_inst 14 RET [] []) = NONE /\
+  raw_return_user_arity (mk_inst 15 RETFMP [] []) = NONE /\
+  raw_return_user_arity (mk_inst 16 DRET [Lit 1w] []) = NONE /\
+  raw_return_user_arity (mk_inst 17 ADD [] []) = NONE
+Proof
+  EVAL_TAC
+QED
+
+Theorem fn_unique_return_arity_eval:
+  fn_unique_return_arity
+    (layout_test_fn
+      [mk_inst 0 RET [Var "u"; Var "rpc"] [];
+       mk_inst 1 RETFMP [Var "u"; Var "rpc"] []] []) = SOME 1 /\
+  fn_unique_return_arity
+    (layout_test_fn
+      [mk_inst 0 RET [Var "u"; Var "rpc"] [];
+       mk_inst 1 RETFMP [Var "u0"; Var "u1"; Var "rpc"] []] []) = NONE /\
+  fn_unique_return_arity
+    (layout_test_fn [mk_inst 0 RET [] []] []) = NONE /\
+  fn_unique_return_arity (layout_test_fn [mk_inst 0 ADD [] []] []) = NONE
+Proof
+  EVAL_TAC
+QED
+
+Theorem fn_return_abi_matches_eval:
+  fn_return_abi_matches
+    (layout_test_fn_with_abi
+      [mk_inst 0 PARAM [Lit 0w] ["retbuf"];
+       mk_inst 1 RET [Var "u"; Var "rpc"] []]
+      [] (SOME T) (SOME 1)) /\
+  ~fn_return_abi_matches
+    (layout_test_fn_with_abi
+      [mk_inst 0 RET [Var "u"; Var "rpc"] []]
+      [] (SOME T) (SOME 1)) /\
+  ~fn_return_abi_matches
+    (layout_test_fn_with_abi
+      [mk_inst 0 PARAM [Lit 0w] ["retbuf"];
+       mk_inst 1 RET [Var "u"; Var "rpc"] []]
+      [] (SOME T) (SOME 2)) /\
+  fn_memory_return_buffer_param
+    (layout_test_fn_with_abi
+      [mk_inst 0 PARAM [Lit 0w] ["retbuf"];
+       mk_inst 1 RET [Var "rpc"] []]
+      [] (SOME T) (SOME 0)) =
+    SOME (mk_inst 0 PARAM [Lit 0w] ["retbuf"])
+Proof
+  EVAL_TAC >> decide_tac
+QED
 val _ = export_theory();
